cleaning and notation for Perm_R

mall.v
@@ -1,3 +1,4 @@
+Require Import Setoid CMorphisms.
 Require Import Lia.
 Require Import PeanoNat.
 
@@ -36,8 +37,8 @@ Fixpoint dual A :=
   match A with
   | var X => covar X
   | covar X => var X
-  | tens A B => parr (dual B) (dual A)
-  | parr A B => tens (dual B) (dual A)
+  | tens A B => parr (dual A) (dual B)
+  | parr A B => tens (dual A) (dual B)
   | aplus A B => awith (dual A) (dual B)
   | awith A B => aplus (dual A) (dual B)
   end.
@@ -48,31 +49,17 @@ Proof. now induction A; simpl; try rewrite IHA1; try rewrite IHA2. Qed.
 Lemma fsize_dual : forall A, fsize (dual A) = fsize A.
 Proof. now induction A; simpl; try rewrite IHA1; try rewrite IHA2; try lia. Qed.
 
-Inductive mll_cut : list formulas -> Type :=
-| ax_cut_r : forall X, mll_cut (covar X :: var X :: nil)
-| ex_cut_r : forall l1 l2, mll_cut l1 -> Perm_R l1 l2 ->
-                             mll_cut l2
-| tens_cut_r : forall A B l1 l2, mll_cut (A :: l1) -> mll_cut (B :: l2) ->
-                                 mll_cut (tens A B :: l2 ++ l1)
-| parr_cut_r : forall A B l, mll_cut (A :: B :: l) -> mll_cut (parr A B :: l)
-| plus_cut_r1 : forall A B l, mll_cut (A :: l) -> mll_cut (aplus A B :: l)
-| plus_cut_r2 : forall A B l, mll_cut (B :: l) -> mll_cut (aplus A B :: l)
-| with_cut_r : forall A B l, mll_cut (A :: l) -> mll_cut (B :: l) ->
-                             mll_cut (awith A B :: l)
-| cut_r : forall A l1 l2, mll_cut (dual A :: l1) -> mll_cut (A :: l2) ->
-                          mll_cut (l2 ++ l1).
-
 Inductive mll : list formulas -> Type :=
 | ax_r : forall X, mll (covar X :: var X :: nil)
-| ex_r : forall l1 l2, mll l1 -> Perm_R l1 l2 ->
-                     mll l2
-| tens_r : forall A B l1 l2, mll (A :: l1) -> mll (B :: l2) ->
-                             mll (tens A B :: l2 ++ l1)
+| ex_r : forall l1 l2, mll l1 -> l1 ~~ l2 -> mll l2
+| tens_r : forall A B l1 l2, mll (A :: l1) -> mll (B :: l2) -> mll (tens A B :: l1 ++ l2)
+| parr_r : forall A B l, mll (A :: B :: l) -> mll (parr A B :: l)
 | plus_r1 : forall A B l, mll (A :: l) -> mll (aplus A B :: l)
 | plus_r2 : forall A B l, mll (B :: l) -> mll (aplus A B :: l)
-| with_r : forall A B l, mll (A :: l) -> mll (B :: l) ->
-                             mll (awith A B :: l)
-| parr_r : forall A B l, mll (A :: B :: l) -> mll (parr A B :: l).
+| with_r : forall A B l, mll (A :: l) -> mll (B :: l) ->  mll (awith A B :: l).
+
+Global Instance Perm_R_mll : Proper (@Perm_R formulas ==> arrow) mll.
+Proof. now intros l1 l2 Hp pi; apply ex_r with l1. Defined.
 
 Fixpoint psize {l} (pi : mll l) :=
   match pi with
@@ -85,19 +72,19 @@ Fixpoint psize {l} (pi : mll l) :=
   | with_r _ _ _ pi1 pi2 => S (psize pi1 + psize pi2)
   end.
 
+Ltac fsize_lia := simpl; rewrite ? fsize_dual; lia.
+
 Lemma cut_admissible : forall A l1 l2,
-  mll (dual A :: l1) -> mll (A :: l2) ->
-    mll (l2 ++ l1).
-Proof with try assumption; try reflexivity.
+  mll (dual A :: l1) -> mll (A :: l2) -> mll (l1 ++ l2).
+Proof with try assumption; try reflexivity; try fsize_lia.
   enough (forall c s A l0 l1 l2 (pi1 : mll (dual A :: l0)) (pi2 : mll (l1 ++ A :: l2)),
           s = psize pi1 + psize pi2 -> fsize A <= c -> mll (l1 ++ l0 ++ l2)) as IH.
   { intros A l1 l2 pi1 pi2.
     rewrite <- (app_nil_l _) in pi2.
-    apply ex_r with (l1 ++ l2); [ | apply Perm_R_app_comm].
     refine (IH _ _ A _ _ _ pi1 pi2 _ _)... }
   induction c as [c IHcut0] using lt_wf_rect.
   assert (forall A, fsize A < c -> forall l0 l1 l2,
-               mll (dual A :: l0) -> mll (l1 ++ A :: l2) -> mll (l1 ++ l0 ++ l2)) as IHcut
+                    mll (dual A :: l0) -> mll (l1 ++ A :: l2) -> mll (l1 ++ l0 ++ l2)) as IHcut
     by (now intros A Hs l0 l1 l2 pi1 pi2 ; refine (IHcut0 _ _ _ _ _ _ _ pi1 pi2 _ _); try eassumption);
     clear IHcut0.
   induction s as [s IHsize0] using lt_wf_rect.
@@ -109,167 +96,169 @@ Proof with try assumption; try reflexivity.
   remember (l1 ++ A :: l2) as l ; destruct pi2.
   - (* ax_r *)
     destruct l1 ; inversion Heql ; subst.
-    + apply ex_r with (var X :: l0); [ | rewrite (Perm_R_app_comm l0)]...
-    + unit_vs_elt_inv H1 ; list_simpl...
+    + simpl; clear - pi1; revert pi1.
+      refine (Perm_R_mll _ _ (Perm_R_cons_append _ _)). (* should be a rewrite Per_R_cons_append, but Coq bug *)
+    + unit_vs_elt_inv H1; list_simpl...
   - (* ex_r *)
     simpl in IHsize; rewrite Heql in p.
     destruct (Perm_R_vs_elt_inv _ _ _ _ p) as [[p1 p2] Heq] ; simpl in Heq ; subst.
-    eapply ex_r ; [ refine (IHsize _ _ _ _ pi1 pi2 _ _) | ]; try lia.
-    apply Perm_R_app_middle; apply Perm_R_app_inv with A...
+    apply ex_r with (p1 ++ l0 ++ p2);
+    [ | now apply Perm_R_app_inv in p; apply Perm_R_app_middle ].
+    refine (IHsize _ _ _ _ pi1 pi2 _ _)...
   - (* tens_r *)
-    destruct l1 ; inversion Heql ; subst ; list_simpl.
+    destruct l1 ; inversion Heql ; subst ; simpl in Hc; list_simpl.
     + (* main case *)
       remember (dual (tens A0 B) :: l0) as l' ; destruct pi1; try inversion Heql'.
       * (* ex_r *)
         remember (tens_r _ _ _ _ pi2_1 pi2_2) as Htens ; clear HeqHtens.
-        revert p IHsize; rewrite Heql'; change (dual (tens A0 B) :: l0) with (nil ++ (dual (tens A0 B) :: l0)); intros p IHsize.
-        destruct (Perm_R_vs_cons_inv _ _ _ p) as [[p1 p2] Heq] ; simpl in Heq ; subst.
-        apply ex_r with (p1 ++ l4 ++ l3 ++ p2).
-        2:{ rewrite <- (app_nil_r (l4 ++ l3)); replace (p1 ++ l4 ++ l3 ++ p2) with (p1 ++ (l4 ++ l3) ++ p2) by (now rewrite<- ? app_assoc).
-            apply Perm_R_app_middle; apply Perm_R_app_inv with (parr (dual B) (dual A0)).
-            rewrite (Perm_R_app_comm l0)... }
-        revert Htens IHsize ; simpl ;
-          replace (tens A0 B) with (dual (parr (dual B) (dual A0)))
-          by (simpl ; rewrite 2 bidual ; reflexivity) ;
+        revert p IHsize; rewrite Heql'; change (dual (tens A0 B) :: l0)
+                                          with (nil ++ (dual (tens A0 B) :: l0)); intros p IHsize.
+        destruct (Perm_R_vs_cons_inv _ _ _ p) as [[p1 p2] Heq] ; simpl in Heq; subst.
+        apply ex_r with (p1 ++ (l3 ++ l4) ++ p2);
+        [ | clear - p; apply Perm_R_app_inv in p; simpl in p; rewrite <- p; list_simpl;
+            apply Perm_R_app_head; now rewrite (Perm_R_app_comm p2); list_simpl ].
+        revert Htens IHsize ; simpl;
+          replace (tens A0 B) with (dual (parr (dual A0) (dual B))) by (now simpl ; rewrite 2 bidual) ;
           intros Htens IHsize.
-        replace (p1 ++ l4 ++ l3 ++ p2) with (p1 ++ (l4 ++ l3) ++ p2) by (now rewrite<- ? app_assoc).
-        refine (IHsize _ _ _ _ Htens pi1 _ _); simpl; simpl in Hc; [ | rewrite 2 fsize_dual]; try lia.
+        refine (IHsize _ _ _ _ Htens pi1 _ _)...
       * (* parr_r *)
         clear IHsize ; subst.
-        rewrite <- (app_nil_l (A0 :: _)) in pi2_1 ; simpl in Hc ; list_simpl.
-        rewrite <- (bidual B) in pi2_2.
+        rewrite <- (bidual A0) in pi2_1; rewrite <- (bidual B) in pi2_2.
+        refine (IHcut _ _ _ _ _ pi2_1 _)...
+        apply ex_r with ((dual A0 :: nil) ++ l4 ++ l0); [ | now rewrite <- Perm_R_app_rot ].
+          (* should be a rewrite Per_R_cons_append, but Coq bug *)
         refine (IHcut _ _ _ _ _ pi2_2 _)...
-        -- rewrite fsize_dual; lia.
-        -- eapply ex_r ; [ | apply Perm_R_app_comm ].
-           list_simpl in pi2_1 ; rewrite <- (bidual A0) in pi2_1.
-           change ((dual B :: l3) ++ l0) with ((dual B :: nil) ++ l3 ++ l0).
-           refine (IHcut _ _ _ _ _ pi2_1 _)...
-           rewrite fsize_dual; lia.
     + (* commutative case *)
       dichot_Type_elt_app_exec H1 ; subst.
       * rewrite 2 app_assoc ; apply tens_r...
-        revert pi2_2 IHsize ; simpl ; rewrite (app_comm_cons _ _ B) ; intros pi2_2 IHsize.
-        rewrite <- app_assoc ; refine (IHsize _ _ _ _ pi1 pi2_2 _ _) ; simpl; lia.
+        revert pi2_1 IHsize ; simpl ; rewrite (app_comm_cons _ _ A0) ; intros pi2_1 IHsize; list_simpl.
+        refine (IHsize _ _ _ _ pi1 pi2_1 _ _)...
       * list_simpl ; apply tens_r...
-        revert pi2_1 IHsize ; simpl ; rewrite (app_comm_cons _ _ A0) ; intros pi2_1 IHsize.
-        refine (IHsize _ _ _ _ pi1 pi2_1 _ _) ; simpl; lia.
+        revert pi2_2 IHsize ; simpl ; rewrite (app_comm_cons _ _ B) ; intros pi2_2 IHsize.
+        refine (IHsize _ _ _ _ pi1 pi2_2 _ _)...
+  - (* parr_r *)
+    destruct l1 ; inversion Heql; subst; simpl in Hc; list_simpl.
+    + (* main case *)
+      remember (dual (parr A0 B) :: l0) as l' ; destruct pi1; try inversion Heql'.
+      * (* ex_r *)
+        remember (parr_r _ _ _ pi2) as Hparr ; clear HeqHparr.
+        revert p IHsize; rewrite Heql'; change (dual (parr A0 B) :: l0)
+                                          with (nil ++ dual (parr A0 B) :: l0); intros p IHsize.
+        destruct (Perm_R_vs_cons_inv _ _ _ p) as [[p1 p2] Heq] ; simpl in Heq ; subst.
+        apply ex_r with (p1 ++ l2 ++ p2);
+        [ | clear - p; apply Perm_R_app_inv in p; simpl in p; rewrite <- p; list_simpl;
+            apply Perm_R_app_head, Perm_R_app_comm ].
+        revert Hparr IHsize ; simpl ;
+          replace (parr A0 B) with (dual (tens (dual A0) (dual B)))
+          by (simpl ; rewrite 2 bidual ; reflexivity) ;
+          intros Hparr IHsize.
+        refine (IHsize _ _ _ _ Hparr pi1 _ _)...
+      * (* tens_r *)
+        clear IHsize ; subst.
+        rewrite <- (app_nil_l (A0 :: _)) in pi2 ; simpl in Hc ; list_simpl.
+        refine (IHcut _ _ _ _ _ pi1_2 _)...
+        rewrite <- (app_nil_l _) ; refine (IHcut _ _ _ _ _ pi1_1 _)...
+    + (* commutative case *)
+      apply parr_r.
+      revert pi2 IHsize ; simpl ; rewrite (app_comm_cons l1 _ B) ; rewrite (app_comm_cons _ _ A0) ;
+        intros pi2 IHsize.
+      refine (IHsize _ _ _ _ pi1 pi2 _ _)...
   - (* plus_r1 *)
-    destruct l1 ; inversion Heql ; subst ; list_simpl.
+    destruct l1; inversion Heql; subst; simpl in Hc; list_simpl.
     + (* main case *)
       remember (dual (aplus A0 B) :: l0) as l' ; destruct pi1; try inversion Heql'.
       * (* ex_r *)
         remember (plus_r1 _ _ _ pi2) as Hplus ; clear HeqHplus.
-        revert p IHsize; rewrite Heql'; change (dual (aplus A0 B) :: l0) with (nil ++ (dual (aplus A0 B)) :: l0); intros p IHsize.
+        revert p IHsize; rewrite Heql'; change (dual (aplus A0 B) :: l0)
+                                          with (nil ++ (dual (aplus A0 B)) :: l0); intros p IHsize.
         destruct (Perm_R_vs_cons_inv _ _ _ p) as [[p1 p2] Heq] ; simpl in Heq ; subst.
-        apply ex_r with (p1 ++ l2 ++ p2).
-        2:{ rewrite<- (app_nil_r l2) at 2.
-            apply Perm_R_app_middle.
-            apply Perm_R_app_inv with (awith (dual A0) (dual B)).
-            rewrite (Perm_R_app_comm l0)... }
+        apply ex_r with (p1 ++ l2 ++ p2);
+        [ | clear - p; apply Perm_R_app_inv in p; simpl in p; rewrite <- p; list_simpl;
+            apply Perm_R_app_head, Perm_R_app_comm ].
         revert Hplus IHsize ; simpl ;
           replace (aplus A0 B) with (dual (awith (dual A0) (dual B)))
           by (simpl ; rewrite 2 bidual ; reflexivity) ;
           intros Hplus IHsize.
-        refine (IHsize _ _ _ _ Hplus pi1 _ _); [ | simpl; rewrite 2 fsize_dual]...
-        lia.
+        refine (IHsize _ _ _ _ Hplus pi1 _ _)...
       * (* with_r *)
         clear IHsize ; subst.
-        rewrite <- (app_nil_l (A0 :: _)) in pi2 ; simpl in Hc ; refine (IHcut _ _ _ _ _ pi1_1 pi2); lia.
+        rewrite <- (app_nil_l (A0 :: _)) in pi2 ; refine (IHcut _ _ _ _ _ pi1_1 pi2)...
     + (* commutative case *)
       apply plus_r1.
       revert pi2 IHsize ; simpl ; rewrite (app_comm_cons l1 _ A0) ; intros pi2 IHsize.
-      refine (IHsize _ _ _ _ pi1 pi2 _ _) ; simpl; lia.
+      refine (IHsize _ _ _ _ pi1 pi2 _ _)...
   - (* plus_r2 *)
-    destruct l1 ; inversion Heql ; subst ; list_simpl.
+    destruct l1; inversion Heql; subst; simpl in Hc; list_simpl.
     + (* main case *)
       remember (dual (aplus A0 B) :: l0) as l' ; destruct pi1; try inversion Heql'.
       * (* ex_r *)
         remember (plus_r2 _ _ _ pi2) as Hplus ; clear HeqHplus.
         revert p IHsize; rewrite Heql'; rewrite<- (app_nil_l (dual (aplus A0 B) :: l0)); intros p IHsize.
         destruct (Perm_R_vs_cons_inv _ _ _ p) as [[p1 p2] Heq] ; simpl in Heq; subst.
-        apply ex_r with (p1 ++ l2 ++ p2).
-        2:{ rewrite<- (app_nil_r l2) at 2.
-            apply Perm_R_app_middle.
-            apply Perm_R_app_inv with (awith (dual A0) (dual B)).
-            rewrite (Perm_R_app_comm l0)... }
+        apply ex_r with (p1 ++ l2 ++ p2);
+        [ | clear - p; apply Perm_R_app_inv in p; simpl in p; rewrite <- p; list_simpl;
+            apply Perm_R_app_head, Perm_R_app_comm ].
         revert Hplus IHsize ; simpl ;
           replace (aplus A0 B) with (dual (awith (dual A0) (dual B)))
           by (simpl ; rewrite 2 bidual ; reflexivity) ;
           intros Hplus IHsize.
-        refine (IHsize _ _ _ _ Hplus pi1 _ _); [ | simpl ; rewrite 2 fsize_dual]...
-        lia.
+        refine (IHsize _ _ _ _ Hplus pi1 _ _)...
       * (* with_r *)
         clear IHsize ; subst.
-        rewrite <- (app_nil_l (B :: _)) in pi2 ; simpl in Hc ; refine (IHcut _ _ _ _ _ pi1_2 pi2); lia.
+        rewrite <- (app_nil_l (B :: _)) in pi2 ; refine (IHcut _ _ _ _ _ pi1_2 pi2)...
     + (* commutative case *)
       apply plus_r2.
       revert pi2 IHsize ; simpl ; rewrite (app_comm_cons l1 _ B) ; intros pi2 IHsize.
-      refine (IHsize _ _ _ _ pi1 pi2 _ _) ; lia.
+      refine (IHsize _ _ _ _ pi1 pi2 _ _)...
   - (* with_r *)
-    destruct l1 ; inversion Heql ; subst ; list_simpl.
+    destruct l1; inversion Heql; subst; simpl in Hc; list_simpl.
     + (* main case *)
       remember (dual (awith A0 B) :: l0) as l' ; destruct pi1 ; try inversion Heql'.
       * (* ex_r *)
         remember (with_r _ _ _ pi2_1 pi2_2) as Hwith ; clear HeqHwith.
-        revert p IHsize; rewrite Heql'; change (dual (awith A0 B) :: l0) with (nil ++ dual (awith A0 B) :: l0); intros p IHsize.
+        revert p IHsize; rewrite Heql'; change (dual (awith A0 B) :: l0)
+                                          with (nil ++ dual (awith A0 B) :: l0); intros p IHsize.
         destruct (Perm_R_vs_cons_inv _ _ _ p) as [[p1 p2] Heq] ; simpl in Heq ; subst.
-        apply ex_r with (p1 ++ l2 ++ p2).
-        2:{ rewrite<- (app_nil_r l2) at 2.
-            apply Perm_R_app_middle.
-            apply Perm_R_app_inv with (aplus (dual A0) (dual B)).
-            rewrite (Perm_R_app_comm l0)... }
+        apply ex_r with (p1 ++ l2 ++ p2);
+        [ | clear - p; apply Perm_R_app_inv in p; simpl in p; rewrite <- p; list_simpl;
+            apply Perm_R_app_head, Perm_R_app_comm ].
         revert Hwith IHsize ; simpl ;
           replace (awith A0 B) with (dual (aplus (dual A0) (dual B)))
           by (simpl ; rewrite 2 bidual ; reflexivity) ;
           intros Hwith IHsize.
-        refine (IHsize _ _ _ _ Hwith pi1 _ _); [ | simpl ; rewrite 2 fsize_dual]...
-        lia.
+        refine (IHsize _ _ _ _ Hwith pi1 _ _)...
       * (* plus_r1 *)
         clear IHsize ; subst.
-        rewrite <- (app_nil_l (A0 :: _)) in pi2_1 ; simpl in Hc ; refine (IHcut _ _ _ _ _ pi1 pi2_1); lia.
+        rewrite <- (app_nil_l (A0 :: _)) in pi2_1; refine (IHcut _ _ _ _ _ pi1 pi2_1)...
       * (* plus_r2 *)
         clear IHsize ; subst.
-        rewrite <- (app_nil_l (B :: _)) in pi2_2 ; simpl in Hc ; refine (IHcut _ _ _ _ _ pi1 pi2_2); lia.
+        rewrite <- (app_nil_l (B :: _)) in pi2_2 ; refine (IHcut _ _ _ _ _ pi1 pi2_2)...
     + (* commutative case *)
       apply with_r.
       * revert pi2_1 IHsize ; simpl ; rewrite (app_comm_cons l1 _ A0) ; intros pi2_1 IHsize.
-        refine (IHsize _ _ _ _ pi1 pi2_1 _ _) ; lia.
+        refine (IHsize _ _ _ _ pi1 pi2_1 _ _)...
       * revert pi2_2 IHsize ; simpl ; rewrite (app_comm_cons l1 _ B) ; intros pi2_2 IHsize.
-        refine (IHsize _ _ _ _ pi1 pi2_2 _ _) ; lia.
-  - (* parr_r *)
-    destruct l1 ; inversion Heql ; subst ; list_simpl.
-    + (* main case *)
-      remember (dual (parr A0 B) :: l0) as l' ; destruct pi1; try inversion Heql'.
-      * (* ex_r *)
-        remember (parr_r _ _ _ pi2) as Hparr ; clear HeqHparr.
-        revert p IHsize; rewrite Heql'; change (dual (parr A0 B) :: l0) with (nil ++ dual (parr A0 B) :: l0); intros p IHsize.
-        destruct (Perm_R_vs_cons_inv _ _ _ p) as [[p1 p2] Heq] ; simpl in Heq ; subst.
-        apply ex_r with (p1 ++ l2 ++ p2).
-        2:{ rewrite<- (app_nil_r l2) at 2.
-            apply Perm_R_app_middle; apply Perm_R_app_inv with (tens (dual B) (dual A0)).
-            rewrite (Perm_R_app_comm l0)... }
-        revert Hparr IHsize ; simpl ;
-          replace (parr A0 B) with (dual (tens (dual B) (dual A0)))
-          by (simpl ; rewrite 2 bidual ; reflexivity) ;
-          intros Hparr IHsize.
-        refine (IHsize _ _ _ _ Hparr pi1 _ _) ; [ | simpl in Hc ; simpl ; rewrite 2 fsize_dual]; lia.
-      * (* tens_r *)
-        clear IHsize ; subst.
-        rewrite <- (app_nil_l (A0 :: _)) in pi2 ; simpl in Hc ; list_simpl.
-        refine (IHcut _ _ _ _ _ pi1_1 _); [lia | ].
-        rewrite <- (app_nil_l _) ; refine (IHcut _ _ _ _ _ pi1_2 _)...
-        lia.
-    + (* commutative case *)
-      apply parr_r.
-      revert pi2 IHsize ; simpl ; rewrite (app_comm_cons l1 _ B) ; rewrite (app_comm_cons _ _ A0) ;
-        intros pi2 IHsize.
-      refine (IHsize _ _ _ _ pi1 pi2 _ _); lia.
+        refine (IHsize _ _ _ _ pi1 pi2_2 _ _)...
 Qed.
 
-Lemma cut_elim : forall l, mll_cut l -> mll l.
-Proof with try assumption.
+
+Inductive mll_cut : list formulas -> Type :=
+| ax_cut_r : forall X, mll_cut (covar X :: var X :: nil)
+| ex_cut_r : forall l1 l2, mll_cut l1 -> l1 ~~ l2 -> mll_cut l2
+| tens_cut_r : forall A B l1 l2, mll_cut (A :: l1) -> mll_cut (B :: l2) -> mll_cut (tens A B :: l1 ++ l2)
+| parr_cut_r : forall A B l, mll_cut (A :: B :: l) -> mll_cut (parr A B :: l)
+| plus_cut_r1 : forall A B l, mll_cut (A :: l) -> mll_cut (aplus A B :: l)
+| plus_cut_r2 : forall A B l, mll_cut (B :: l) -> mll_cut (aplus A B :: l)
+| with_cut_r : forall A B l, mll_cut (A :: l) -> mll_cut (B :: l) -> mll_cut (awith A B :: l)
+| cut_r : forall A l1 l2, mll_cut (dual A :: l1) -> mll_cut (A :: l2) ->  mll_cut (l1 ++ l2).
+
+Global Instance Perm_R_mll_cut : Proper (@Perm_R formulas ==> arrow) mll_cut.
+Proof. now intros l1 l2 Hp pi; apply ex_cut_r with l1. Defined.
+
+Theorem cut_elim : forall l, mll_cut l -> mll l.
+Proof.
   intros l pi.
   induction pi; try (now constructor); try (eapply ex_r; eassumption).
-  apply cut_admissible with A...
+  now apply cut_admissible with A.
 Qed.
 
