Perm_R.v
@@ -19,9 +19,13 @@ Set Implicit Arguments.
 Definition Perm_R {A} (l1 l2 : list A) : Type :=
   { p : _ & is_perm p = true & prod (length p = length l1) (l2 = app_nat_fun p l1) }.
 
+Infix "~~" := Perm_R (at level 70).
+
+Definition Perm_R_to_perm {A} {l1 l2 : list A} : Perm_R l1 l2 -> perm := @sigT_of_sigT2 _ _ _.
+
 (* Permutation over lists is an equivalence relation *)
 
-Lemma Perm_R_refl {A} : forall (l : list A), Perm_R l l.
+Lemma Perm_R_refl {A} : forall (l : list A), l ~~ l.
 Proof.
   intro l; split with (Id (length l)); repeat split.
   - apply Id_is_perm.
@@ -29,8 +33,7 @@ Proof.
   - symmetry; apply app_Id.
 Defined.
 
-Lemma Perm_R_trans {A} : forall (l1 l2 l3 : list A),
-  Perm_R l1 l2 -> Perm_R l2 l3 -> Perm_R l1 l3.
+Lemma Perm_R_trans {A} : forall (l1 l2 l3 : list A), l1 ~~ l2 -> l2 ~~ l3 -> l1 ~~ l3.
 Proof.
   intros l1 l2 l3 [p1 Hperm1 [Hlen1 IHHp1]] [p2 Hperm2 [Hlen2 IHHp2]].
   assert (length p2 = length p1) by (now rewrite Hlen2, IHHp1; apply app_nat_fun_length).
@@ -43,7 +46,7 @@ Proof.
     now rewrite<- IHHp1.
 Defined.
 
-Lemma Perm_R_sym {A} : forall (l1 l2 : list A), Perm_R l1 l2 -> Perm_R l2 l1.
+Lemma Perm_R_sym {A} : forall (l1 l2 : list A), l1 ~~ l2 -> l2 ~~ l1.
 Proof.
   intros l1 l2 [p Hperm [Hlen Heq]].
   destruct (perm_inv p Hperm) as [p_inv [Heq_inv _ ] [Hperm_inv Hlen_eq]].
@@ -68,14 +71,13 @@ Context {A : Type}.
 Implicit Types a b : A.
 Implicit Types l m : list A.
 
-Lemma Perm_R_nil : forall l, Perm_R nil l -> l = nil.
+Lemma Perm_R_nil : forall l, nil ~~ l -> l = nil.
 Proof. intros l Hperm; destruct Hperm as [f Hp [Hlen Heq]]; now rewrite Heq. Qed.
 
-Lemma Perm_R_nil_cons : forall l a, Perm_R nil (a :: l) -> False.
+Lemma Perm_R_nil_cons : forall l a, nil ~~ (a :: l) -> False.
 Proof. intros l a Hp; apply Perm_R_nil in Hp; inversion Hp. Qed.
 
-Theorem Perm_R_app : forall l m l' m',
- Perm_R l l' -> Perm_R m m' -> Perm_R (l ++ m) (l' ++ m').
+Theorem Perm_R_app : forall l m l' m', l ~~ l' -> m ~~ m' -> l ++ m ~~ l' ++ m'.
 Proof.
 intros l m l' m' [p Hperm [Hlen Heq]] [p' Hperm' [Hlen' Heq']].
 split with (p ++ incr_all p' (length p)); repeat split.
@@ -89,16 +91,13 @@ Defined.
 Global Instance Perm_R_app' : Proper (@Perm_R A ==> @Perm_R A ==> @Perm_R A) (@app A) | 10.
 Proof. repeat intro; now apply Perm_R_app. Defined.
 
-Lemma Perm_R_app_tail : forall l l' tl,
-  Perm_R l l' -> Perm_R (l ++ tl) (l' ++ tl).
+Lemma Perm_R_app_tail : forall l l' tl, l ~~ l' -> l ++ tl ~~ l' ++ tl.
 Proof. intros; now apply Perm_R_app. Defined.
 
-Lemma Perm_R_app_head : forall l tl tl',
- Perm_R tl tl' -> Perm_R (l ++ tl) (l ++ tl').
+Lemma Perm_R_app_head : forall l tl tl', tl ~~ tl' -> l ++ tl ~~ l ++ tl'.
 Proof. intros; now apply Perm_R_app. Defined.
 
-Lemma Perm_R_skip : forall l l' a,
-  Perm_R l l' -> Perm_R (a :: l) (a :: l').
+Lemma Perm_R_skip : forall l l' a, l ~~ l' -> a :: l ~~ a :: l'.
 Proof.
 intros l l' a HP.
 change (a :: l) with ((a :: nil) ++ l).
@@ -109,8 +108,7 @@ Defined.
 Instance Perm_R_cons : Proper (Logic.eq ==> @Perm_R A ==> @Perm_R A) (@cons A) | 10.
 Proof. repeat intro; subst; now apply Perm_R_skip. Defined.
 
-Lemma Perm_R_swap : forall l a b,
-  Perm_R (a :: b :: l) (b :: a :: l).
+Lemma Perm_R_swap : forall l a b, a :: b :: l ~~ b :: a :: l.
 Proof.
 intros l a b.
 change (a :: b :: l) with ((a :: b :: nil) ++ l).
@@ -122,20 +120,16 @@ Defined.
 
 (* Compatibility with others operations on lists *)
 
-Lemma Perm_R_length : forall l m,
-  Perm_R l m -> length l = length m.
+Lemma Perm_R_length : forall l m, l ~~ m -> length l = length m.
 Proof. intros l m [f Hp [Hlen Heq]]; subst; now rewrite app_nat_fun_length. Qed.
 
 Global Instance Perm_R_length' : Proper (@Perm_R A ==> Logic.eq) (@length A) | 10.
 Proof. exact Perm_R_length. Qed.
 
-Lemma Perm_R_add_inside : forall a l l' tl tl',
-  Perm_R l l' -> Perm_R tl tl' ->
-  Perm_R (l ++ a :: tl) (l' ++ a :: tl').
+Lemma Perm_R_add_inside : forall a l l' tl tl', l ~~ l' -> tl ~~ tl' -> l ++ a :: tl ~~ l' ++ a :: tl'.
 Proof. intros; now apply Perm_R_app; [ | apply Perm_R_skip ]. Defined.
 
-Theorem Perm_R_app_comm : forall l l',
-  Perm_R (l ++ l') (l' ++ l).
+Theorem Perm_R_app_comm : forall l l', l ++ l' ~~ l' ++ l.
 Proof.
 intros l l'.
 split with (cfun (length l) (length l')); repeat split.
@@ -144,33 +138,28 @@ split with (cfun (length l) (length l')); repeat split.
 - now rewrite app_cfun_eq.
 Defined.
 
-Lemma Perm_R_cons_append : forall l a,
-  Perm_R (a :: l) (l ++ a :: nil).
+Lemma Perm_R_cons_append : forall l a, a :: l ~~ l ++ a :: nil.
 Proof. intros l a; change (a :: l) with ((a :: nil) ++ l); apply Perm_R_app_comm. Defined.
 
-Theorem Perm_R_middle : forall l1 l2 a,
-  Perm_R (a :: l1 ++ l2) (l1 ++ a :: l2).
+Theorem Perm_R_middle : forall l1 l2 a, a :: l1 ++ l2 ~~ l1 ++ a :: l2.
 Proof. intros; now rewrite Perm_R_app_comm, app_comm_cons, Perm_R_app_comm. Defined.
 
-Theorem Perm_R_cons_app : forall l l1 l2 a,
-  Perm_R l (l1 ++ l2) -> Perm_R (a :: l) (l1 ++ a :: l2).
+Theorem Perm_R_cons_app : forall l l1 l2 a, l ~~ l1 ++ l2 -> a :: l ~~ l1 ++ a :: l2.
 Proof. intros l l1 l2 a Hperm; rewrite Hperm; apply Perm_R_middle. Defined.
 
-Lemma Perm_R_Add_Type a l l' : Add_Type a l l' -> Perm_R (a :: l) l'.
+Lemma Perm_R_Add_Type a l l' : Add_Type a l l' -> a :: l ~~ l'.
 Proof. intros Hadd; induction Hadd; [ reflexivity | rewrite <- IHHadd; apply Perm_R_swap ]. Defined.
 
-Theorem Perm_R_rev : forall l, Perm_R l (rev l).
+Theorem Perm_R_rev : forall l, l ~~ rev l.
 Proof. induction l; [ reflexivity | simpl; rewrite <- IHl; apply Perm_R_cons_append ]. Defined.
 
 Global Instance Perm_R_rev' : Proper (@Perm_R A ==> @Perm_R A) (@rev A) | 10.
 Proof. repeat intro; now rewrite <- 2 Perm_R_rev. Defined.
 
-Theorem Perm_R_nil_app_cons : forall l m a,
-  Perm_R nil (l ++ a :: m) -> False.
+Theorem Perm_R_nil_app_cons : forall l m a, nil ~~ l ++ a :: m -> False.
 Proof. intros l l' a Hperm; rewrite <- Perm_R_middle in Hperm; apply (Perm_R_nil_cons Hperm). Qed.
 
-Theorem Perm_R_cons_inv l l' a :
-  Perm_R (a :: l) (a :: l') -> Perm_R l l'.
+Theorem Perm_R_cons_inv l l' a : a :: l ~~ a :: l' -> l ~~ l'.
 Proof with try assumption; try reflexivity.
 intros [p Hperm [Hlen Heq]].
 destruct p; [ inversion Heq | ].
@@ -191,7 +180,7 @@ rewrite Heql, app_nat_fun_downshift...
 Defined.
 
 Theorem Perm_R_Add_Type_inv a l1 l2 : Perm_R l1 l2 ->
-  forall l1' l2', Add_Type a l1' l1 -> Add_Type a l2' l2 -> Perm_R l1' l2'.
+  forall l1' l2', Add_Type a l1' l1 -> Add_Type a l2' l2 -> l1' ~~ l2'.
 Proof.
 intros Hperm l1' l2' Hadd1 Hadd2.
 apply Perm_R_cons_inv with a.
@@ -199,30 +188,19 @@ transitivity l1; [ now apply Perm_R_Add_Type | ].
 transitivity l2; [ apply Hperm | now symmetry; apply Perm_R_Add_Type ].
 Defined.
 
-Theorem Perm_R_app_inv l1 l2 l3 l4 a :
-  Perm_R (l1 ++ a :: l2) (l3 ++ a :: l4) -> Perm_R (l1 ++ l2) (l3 ++ l4).
-Proof.
-intros Hperm.
-apply Perm_R_cons_inv with a.
-etransitivity; [ now apply Perm_R_middle | ].
-etransitivity; [ apply Hperm | now symmetry; apply Perm_R_middle ].
-Defined.
+Theorem Perm_R_app_inv l1 l2 l3 l4 a : l1 ++ a :: l2 ~~ l3 ++ a :: l4 -> l1 ++ l2 ~~l3 ++ l4.
+Proof. intros; apply Perm_R_cons_inv with a; now rewrite 2 Perm_R_middle. Defined.
 
-Theorem Perm_R_cons_app_inv l l1 l2 a :
-  Perm_R (a :: l) (l1 ++ a :: l2) -> Perm_R l (l1 ++ l2).
+Theorem Perm_R_cons_app_inv l l1 l2 a : a :: l ~~ l1 ++ a :: l2 -> l ~~ l1 ++ l2.
 Proof. intros Hperm; rewrite <- (app_nil_l l); now apply Perm_R_app_inv with a. Defined.
 
-Theorem Perm_R_app_inv_l : forall l l1 l2,
-  Perm_R (l ++ l1) (l ++ l2) -> Perm_R l1 l2.
+Theorem Perm_R_app_inv_l : forall l l1 l2, l ++ l1 ~~ l ++ l2 -> l1 ~~ l2.
 Proof. now induction l; intros l1 l2 Hperm; [ | apply IHl; apply Perm_R_cons_inv with a]. Defined.
 
-Theorem Perm_R_app_inv_r l l1 l2 :
-  Perm_R (l1 ++ l) (l2 ++ l) -> Perm_R l1 l2.
-Proof.
-  now induction l; intros Hperm; [ rewrite 2 app_nil_r in Hperm | apply IHl; apply Perm_R_app_inv with a].
-Defined.
+Theorem Perm_R_app_inv_r l l1 l2 : l1 ++ l ~~ l2 ++ l -> l1 ~~ l2.
+Proof. intros Hperm; rewrite 2 (Perm_R_app_comm _ l) in Hperm; apply (Perm_R_app_inv_l _ _ _ Hperm). Defined.
 
-Lemma Perm_R_length_1_inv: forall a l, Perm_R (a :: nil) l -> l = (a :: nil).
+Lemma Perm_R_length_1_inv: forall a l, a :: nil ~~ l -> l = a :: nil.
 Proof.
 intros a l [p Hperm [Hlen Heq]].
 destruct p; try now inversion Hlen.
@@ -231,15 +209,11 @@ rewrite Heq; simpl.
 now destruct n.
 Qed.
 
-Lemma Perm_R_length_1: forall a b, Perm_R (a :: nil) (b :: nil) -> a = b.
-Proof.
-intros a b Hperm.
-apply Perm_R_length_1_inv in Hperm.
-now inversion Hperm.
-Qed.
+Lemma Perm_R_length_1: forall a b, a :: nil ~~ b :: nil -> a = b.
+Proof. intros a b Hperm; apply Perm_R_length_1_inv in Hperm; now inversion Hperm. Qed.
 
 Lemma Perm_R_length_2_inv : forall a1 a2 l,
-  Perm_R (a1 :: a2 :: nil) l -> { l = a1 :: a2 :: nil } + { l = a2 :: a1 :: nil }.
+  a1 :: a2 :: nil ~~ l -> { l = a1 :: a2 :: nil } + { l = a2 :: a1 :: nil }.
 Proof.
 intros a1 a2 l [p Hperm [Hlen Heq]].
 do 3 (destruct p; try now inversion Hlen).
@@ -247,13 +221,13 @@ now apply is_perm_length_2_inv in Hperm as [[Hp1 Hp2] | [Hp1 Hp2]]; subst; simpl
 Defined.
 
 Lemma Perm_R_length_2 : forall a1 a2 b1 b2,
-  Perm_R (a1 :: a2 :: nil) (b1 :: b2 :: nil) -> { a1 = b1 /\ a2 = b2 } + { a1 = b2 /\ a2 = b1 }.
+  a1 :: a2 :: nil ~~ b1 :: b2 :: nil -> { a1 = b1 /\ a2 = b2 } + { a1 = b2 /\ a2 = b1 }.
 Proof.
 intros a1 a2 b1 b2 Hperm.
 now destruct (Perm_R_length_2_inv Hperm) as [Heq | Heq]; inversion Heq; subst; [left | right].
 Defined.
 
-Theorem Perm_R_in : forall l m a, Perm_R l m -> In a l -> In a m.
+Theorem Perm_R_in : forall l m a, l ~~ m -> In a l -> In a m.
 Proof.
 intros l m a [p Hperm [Hlen Heq]] Hin.
 apply In_nth with _ _ _ a in Hin as [n (Hlen' & Heq')].
@@ -269,7 +243,7 @@ Qed.
 Global Instance Perm_R_in' : Proper (Logic.eq ==> @Perm_R A ==> iff) (@In A) | 10.
 Proof. repeat intro; subst; split; now apply Perm_R_in. Qed.
 
-Theorem Perm_R_in_Type : forall l m a, Perm_R l m -> In_Type a l -> In_Type a m.
+Theorem Perm_R_in_Type : forall l m a, l ~~ m -> In_Type a l -> In_Type a m.
 Proof.
 intros l m a [p Hperm [Hlen Heq]] Hin.
 apply In_nth_Type with _ _ a in Hin as [n Hlen' Heq'].
@@ -292,7 +266,7 @@ Section Perm_R_map.
 Variable A B : Type.
 Variable f : A -> B.
 
-Lemma Perm_R_map l l' : Perm_R l l' -> Perm_R (map f l) (map f l').
+Lemma Perm_R_map l l' : l ~~ l' -> map f l ~~ map f l'.
 Proof.
   intros [p Hperm [Hlen Heq]].
   split with p; repeat split; [ assumption | | ].
@@ -305,14 +279,15 @@ Proof. exact Perm_R_map. Defined.
 
 End Perm_R_map.
 
+
 (* INDUCTION PRINCIPLE *)
 Theorem Perm_R_rect_transpo {A} :
  forall P : list A -> list A -> Type,
    P nil nil ->
-   (forall x l l', Perm_R l l' -> P l l' -> P (x :: l) (x :: l')) ->
+   (forall x l l', l ~~ l' -> P l l' -> P (x :: l) (x :: l')) ->
    (forall x y l, P (y :: x :: l) (x :: y :: l)) ->
-   (forall l l' l'', Perm_R l l' -> P l l' -> Perm_R l' l'' -> P l' l'' -> P l l'') ->
-   forall l l', Perm_R l l' -> P l l'.
+   (forall l l' l'', l ~~ l' -> P l l' -> l' ~~ l'' -> P l' l'' -> P l l'') ->
+   forall l l', l ~~ l' -> P l l'.
 Proof with try assumption; try reflexivity.
   intros P Hnil Hskip Hswap Htrans.
   intros l l' Hperm.
@@ -408,10 +383,10 @@ Ltac rect_transpo P Hperm :=
 Theorem Perm_R_ind_transpo {A} :
  forall P : list A -> list A -> Prop,
    P nil nil ->
-   (forall x l l', Perm_R l l' -> P l l' -> P (x :: l) (x :: l')) ->
+   (forall x l l', l ~~ l' -> P l l' -> P (x :: l) (x :: l')) ->
    (forall x y l, P (y :: x :: l) (x :: y :: l)) ->
-   (forall l l' l'', Perm_R l l' -> P l l' -> Perm_R l' l'' -> P l' l'' -> P l l'') ->
-   forall l l', Perm_R l l' -> P l l'.
+   (forall l l' l'', l ~~ l' -> P l l' -> l' ~~ l'' -> P l' l'' -> P l l'') ->
+   forall l l', l ~~ l' -> P l l'.
 Proof. intros; now apply Perm_R_rect_transpo. Qed.
 
 Ltac ind_transpo P Hperm :=
@@ -427,19 +402,29 @@ Ltac ind_transpo P Hperm :=
   refine (Perm_R_rect_transpo P  _ _ _ _ Hperm); clear Hperm;
   [ | intros x la lb Hperm1 IHHperm1 | intros x y la | intros la lb lc Hperm1 IHHperm1 Hperm2 IHHperm2].
 
+Theorem Perm_R_rect_transpo_bis {A} :
+ forall P : list A -> list A -> Type,
+   P nil nil ->
+   (forall x l l', l ~~ l' -> P l l' -> P (x :: l) (x :: l')) ->
+   (forall x y l l', l ~~ l' -> P l l' -> P (y :: x :: l) (x :: y :: l')) ->
+   (forall l l' l'', l ~~ l' -> P l l' -> l' ~~ l'' -> P l' l'' -> P l l'') ->
+   forall l l', l ~~ l' -> P l l'.
+Proof.
+  intros P Hnil Hskip Hswap Htrans.
+  assert (forall l, P l l) as Hrefl by (now induction l; [ | apply Hskip; [ reflexivity | ] ]).
+  apply Perm_R_rect_transpo; try assumption.
+  now intros x y l; apply Hswap.
+Qed.
+
+
 Theorem Perm_R_ind_transpo_bis {A} :
  forall P : list A -> list A -> Prop,
    P nil nil ->
-   (forall x l l', Perm_R l l' -> P l l' -> P (x :: l) (x :: l')) ->
-   (forall x y l l', Perm_R l l' -> P l l' -> P (y :: x :: l) (x :: y :: l')) ->
-   (forall l l' l'', Perm_R l l' -> P l l' -> Perm_R l' l'' -> P l' l'' -> P l l'') ->
-   forall l l', Perm_R l l' -> P l l'.
-Proof.
-intros P Hnil Hskip Hswap Htrans.
-assert (forall l, P l l) as Hrefl by (now induction l; [ | apply Hskip; [ reflexivity | ] ]).
-apply Perm_R_rect_transpo; try assumption.
-now intros x y l; apply Hswap.
-Qed.
+   (forall x l l', l ~~ l' -> P l l' -> P (x :: l) (x :: l')) ->
+   (forall x y l l', l ~~ l' -> P l l' -> P (y :: x :: l) (x :: y :: l')) ->
+   (forall l l' l'', l ~~ l' -> P l l' -> l' ~~ l'' -> P l' l'' -> P l l'') ->
+   forall l l', l ~~ l' -> P l l'.
+Proof. intros; now apply Perm_R_rect_transpo_bis. Qed.
 
 Ltac ind_transpo_bis P Hperm :=
   let x := fresh "x" in
@@ -454,19 +439,6 @@ Ltac ind_transpo_bis P Hperm :=
   refine (Perm_R_ind_transpo_bis P  _ _ _ _ Hperm); clear Hperm;
   [ | intros x la lb Hperm1 IHHperm1 | intros x y la | intros la lb lc Hperm1 IHHperm1 Hperm2 IHHperm2].
 
-Theorem Perm_R_rect_transpo_bis {A} :
- forall P : list A -> list A -> Type,
-   P nil nil ->
-   (forall x l l', Perm_R l l' -> P l l' -> P (x :: l) (x :: l')) ->
-   (forall x y l l', Perm_R l l' -> P l l' -> P (y :: x :: l) (x :: y :: l')) ->
-   (forall l l' l'', Perm_R l l' -> P l l' -> Perm_R l' l'' -> P l' l'' -> P l l'') ->
-   forall l l', Perm_R l l' -> P l l'.
-Proof.
-  intros P Hnil Hskip Hswap Htrans.
-  assert (forall l, P l l) as Hrefl by (now induction l; [ | apply Hskip; [ reflexivity | ] ]).
-  apply Perm_R_rect_transpo; try assumption.
-  now intros x y l; apply Hswap.
-Qed.
 
 Ltac rect_transpo_bis P Hperm :=
   let x := fresh "x" in
@@ -488,7 +460,7 @@ Ltac rect_transpo_bis P Hperm :=
 Require Import Permutation_Type_solve.
 
 Lemma Permutation_Type_to_Perm_R {A} : forall l1 (l2 : list A),
-  Permutation_Type l1 l2 -> Perm_R l1 l2.
+  Permutation_Type l1 l2 -> l1 ~~ l2.
 Proof.
 intros l1 l2 Hp; induction Hp.
 - now split with (Id 0); repeat split.
@@ -498,7 +470,7 @@ intros l1 l2 Hp; induction Hp.
 Defined.
 
 Lemma Perm_R_to_Permutation_Type {A} : forall (l1 : list A) l2,
-  Perm_R l1 l2 -> Permutation_Type l1 l2.
+  l1 ~~ l2 -> Permutation_Type l1 l2.
 Proof.
 intros l1 l2 Hperm.
 apply Perm_R_rect_transpo; (try now (intros; constructor)); [ | assumption ].
